theories/Factor_Proof_Node_Construction.thy
@@ -4,6 +4,148 @@ begin
 
 section \<open>Complete finite syntax for inference metadata\<close>
 
+locale inference_node_syntax_construction =
+  fixes d :: "local_address option definition_site"
+    and V :: "(local_address option definition_site\<times>factor_term) fset"
+    and D :: "(local_address option definition_site\<times>local_address option definition_site) set"
+    and Rb Rp :: exact_artifact
+    and Lb Lp :: "(local_address\<times>exact_artifact) set"
+    and Cb Cp :: "(local_address\<times>local_address option definition_site) set"
+    and Ib Kb Ip Kp :: "local_address set"
+  assumes address: "octets_formed (snd d)"
+    and b: "exact_formed Rb" "bag_count (object_data Rb)=(\<lambda>_. 0)"
+      "[]\<in>rra_carrier (object_structure Rb)" "reference_table_formed Lb Cb"
+      "rra_carrier (object_structure Rb)=Ib\<union>Kb" "Ib\<inter>Kb={}"
+      "Kb=rel_dom Lb\<union>rel_dom Cb" "rel_ran Cb=rel_dom (fset V)"
+      "\<forall>E u. environment_formed E \<longrightarrow> artifact_at E u Rb \<longrightarrow> syntax_references E u Lb Cb \<longrightarrow>
+        native_binding_table_at E u [] (fset V) Ib Kb"
+    and p: "exact_formed Rp" "bag_count (object_data Rp)=(\<lambda>_. 0)"
+      "[]\<in>rra_carrier (object_structure Rp)" "reference_table_formed Lp Cp"
+      "rra_carrier (object_structure Rp)=Ip\<union>Kp" "Ip\<inter>Kp={}"
+      "Kp=rel_dom Lp\<union>rel_dom Cp" "rel_ran Cp=rel_dom D\<union>rel_ran D"
+      "\<forall>E u. environment_formed E \<longrightarrow> artifact_at E u Rp \<longrightarrow> syntax_references E u Lp Cp \<longrightarrow>
+        native_discharge_table_at E u [] D Ip Kp"
+begin
+
+abbreviation clause_syntax where "clause_syntax \<equiv> external_occurrence_syntax (snd d)"
+abbreviation clause_interior :: "local_address set" where "clause_interior \<equiv> {[],[5]}"
+abbreviation clause_slots :: "local_address set" where "clause_slots \<equiv> {[4]}"
+abbreviation callees where "callees \<equiv> [{([4],d)},Cb,Cp]"
+abbreviation literals where "literals \<equiv> [{},Lb,Lp]"
+abbreviation interiors where "interiors \<equiv> [clause_interior,Ib,Ip]"
+abbreviation slots where "slots \<equiv> [clause_slots,Kb,Kp]"
+abbreviation artifacts where "artifacts \<equiv> [clause_syntax,Rb,Rp]"
+
+lemma cf: "exact_formed clause_syntax" by (rule external_occurrence_syntax_formed[OF address])
+lemma profile: "reference_table_formed {} {([4],d)}"
+    by (rule reference_table_callees) (simp_all add: single_valued_def)
+lemma cc: "rra_carrier (object_structure clause_syntax)=clause_interior\<union>clause_slots"
+    by (auto simp: external_occurrence_syntax_def)
+lemma cs: "clause_interior\<inter>clause_slots={}" by auto
+lemma cd: "clause_slots=rel_dom ({} :: (local_address\<times>exact_artifact) set)\<union>rel_dom {([4],d)}"
+    by (auto simp: rel_dom_def)
+sublocale assembled: record_syntax_construction artifacts interiors slots literals callees
+  proof (rule record_syntax_construction.intro)
+    show "\<forall>R\<in>set artifacts. exact_formed R" using cf b(1) p(1) by simp
+    show "\<forall>R\<in>set artifacts. bag_count (object_data R)=(\<lambda>_. 0)"
+      using b(2) p(2) external_occurrence_syntax_properties(2) by simp
+    show "\<forall>R\<in>set artifacts. []\<in>rra_carrier (object_structure R)"
+      using b(3) p(3) external_occurrence_syntax_properties(1) by simp
+    show "length interiors=length artifacts" "length slots=length artifacts"
+      "length literals=length artifacts" "length callees=length artifacts" by simp_all
+    show "\<forall>i<length artifacts. rra_carrier (object_structure (artifacts!i))=interiors!i\<union>slots!i"
+      using cc b(5) p(5) by (auto simp: less_Suc_eq)
+    show "\<forall>i<length artifacts. interiors!i\<inter>slots!i={}"
+      using cs b(6) p(6) by (auto simp: less_Suc_eq)
+    show "\<forall>i<length artifacts. slots!i=rel_dom (literals!i)\<union>rel_dom (callees!i)"
+      using cd b(7) p(7) by (auto simp: less_Suc_eq)
+    show "\<forall>i<length artifacts. reference_table_formed (literals!i) (callees!i)"
+      using profile b(4) p(4) by (auto simp: less_Suc_eq)
+  qed
+lemma br: "rel_dom Lb\<union>rel_dom Cb\<subseteq>rra_carrier (object_structure Rb)" using b(5,7) by blast
+lemma pr: "rel_dom Lp\<union>rel_dom Cp\<subseteq>rra_carrier (object_structure Rp)" using p(5,7) by blast
+lemma bd: "rel_dom (fset V)\<subseteq>rel_ran Cb" using b(8) by simp
+lemma pd: "rel_dom D\<union>rel_ran D\<subseteq>rel_ran Cp" using p(8) by simp
+lemma cite_range: "rel_ran {([4],d)}={d}" by (auto simp: rel_ran_def)
+lemma deps: "rel_ran assembled.callees=insert d (rel_dom (fset V)\<union>rel_dom D\<union>rel_ran D)"
+    using assembled.reference_range by (simp add: cite_range b(8) p(8) Un_assoc)
+lemma recover: "\<forall>E u. environment_formed E \<longrightarrow> artifact_at E u assembled.framed \<longrightarrow>
+      syntax_references E u assembled.literals assembled.callees \<longrightarrow>
+      native_proof_node_at E u [] (Schema_Inference d V) D assembled.interior assembled.slots"
+  proof (intro allI impI)
+    fix E u assume ef: "environment_formed E" and art: "artifact_at E u assembled.framed"
+      and refs: "syntax_references E u assembled.literals assembled.callees"
+    have caddr: "finite_addressing (rra_carrier (object_structure clause_syntax)) (syntax_branch 0)"
+      using assembled.child_addressing[of 0] by simp
+    have cread: "object_reads_agree (push_object (syntax_branch 0) clause_syntax) assembled.framed
+      (image (syntax_branch 0) (rra_carrier (object_structure clause_syntax)))"
+      using assembled.frame.record_child_reads[of 0] by simp
+    have centry: "(syntax_branch 0 [4],d)\<in>assembled.callees"
+      by (rule syntax_forest_table_member[where i=0]) simp_all
+    have cite: "site_citation_at E u (syntax_branch 0 []) d (image (syntax_branch 0) clause_interior) {syntax_branch 0 [4]}"
+      by (rule external_syntax_embedded_site[OF ef art address caddr cread refs centry])
+    have baddr: "finite_addressing (rra_carrier (object_structure Rb)) (syntax_branch 1)"
+      using assembled.child_addressing[of 1] by simp
+    have bread: "object_reads_agree (push_object (syntax_branch 1) Rb) assembled.framed
+      (image (syntax_branch 1) (rra_carrier (object_structure Rb)))"
+      using assembled.frame.record_child_reads[of 1] by simp
+    have brefs: "syntax_references E u (map_slot_keys (syntax_branch 1) Lb) (map_slot_keys (syntax_branch 1) Cb)"
+      using assembled.child_references[OF refs, of 1] by simp
+    have binding_read: "native_binding_table_at E u (syntax_branch 1 []) (fset V)
+      (image (syntax_branch 1) Ib) (image (syntax_branch 1) Kb)"
+      by (rule compiled_binding_table_embedded[OF b(1) br b(9)[rule_format] bd ef art
+          syntax_branch_injective baddr bread brefs])
+    have paddr: "finite_addressing (rra_carrier (object_structure Rp)) (syntax_branch 2)"
+      using assembled.child_addressing[of 2] by simp
+    have pread: "object_reads_agree (push_object (syntax_branch 2) Rp) assembled.framed
+      (image (syntax_branch 2) (rra_carrier (object_structure Rp)))"
+      using assembled.frame.record_child_reads[of 2] by simp
+    have prefs: "syntax_references E u (map_slot_keys (syntax_branch 2) Lp) (map_slot_keys (syntax_branch 2) Cp)"
+      using assembled.child_references[OF refs, of 2] by simp
+    have discharge_read: "native_discharge_table_at E u (syntax_branch 2 []) D
+      (image (syntax_branch 2) Ip) (image (syntax_branch 2) Kp)"
+      by (rule compiled_discharge_table_embedded[OF p(1) pr p(9)[rule_format] pd ef art
+          syntax_branch_injective paddr pread prefs])
+    let ?C = "image (syntax_branch 0) clause_interior"
+    let ?B = "image (syntax_branch 1) Ib"
+    let ?P = "image (syntax_branch 2) Ip"
+    let ?A = "{syntax_branch 0 [4]}"
+    let ?L = "image (syntax_branch 1) Kb"
+    let ?W = "image (syntax_branch 2) Kp"
+    have rec: "record_at assembled.framed [] assembled.frame.ports
+      [syntax_branch 0 [],syntax_branch 1 [],syntax_branch 2 []]"
+      using assembled.frame.record_read by (simp add: upt_conv_Cons numeral_2_eq_2)
+    have header: "insert [] (set assembled.frame.ports)\<inter>(?C\<union>?B\<union>?P)={}"
+      using assembled.header_separate by (simp add: syntax_forest_three_positions Un_assoc)
+    have cb: "?C\<inter>?B={}" using assembled.child_interiors_separate[of 0 1] by simp
+    have cp: "?C\<inter>?P={}" using assembled.child_interiors_separate[of 0 2] by simp
+    have bp: "?B\<inter>?P={}" using assembled.child_interiors_separate[of 1 2] by simp
+    have separate: "insert [] (set assembled.frame.ports\<union>?C\<union>?B\<union>?P)\<inter>(?A\<union>?L\<union>?W)={}"
+      using assembled.boundary by (simp add: syntax_forest_three_positions Un_assoc)
+    have native: "native_proof_node_at E u [] (Schema_Inference d V) D
+      (insert [] (set assembled.frame.ports\<union>?C\<union>?B\<union>?P)) (?A\<union>?L\<union>?W)"
+      by (rule native_proof_node_at.inference[OF ef art rec cite binding_read discharge_read header cb cp bp separate])
+    show "native_proof_node_at E u [] (Schema_Inference d V) D assembled.interior assembled.slots"
+      using native by (simp add: syntax_forest_three_positions Un_assoc)
+  qed
+theorem total:
+  "\<exists>R L C I K. exact_formed R \<and> bag_count (object_data R)=(\<lambda>_. 0) \<and>
+    []\<in>rra_carrier (object_structure R) \<and> reference_table_formed L C \<and>
+    rra_carrier (object_structure R)=I\<union>K \<and> I\<inter>K={} \<and>
+    K=rel_dom L\<union>rel_dom C \<and>
+    rel_ran C=insert d (rel_dom (fset V)\<union>rel_dom D\<union>rel_ran D) \<and>
+    (\<forall>E u. environment_formed E \<longrightarrow> artifact_at E u R \<longrightarrow> syntax_references E u L C \<longrightarrow>
+      native_proof_node_at E u [] (Schema_Inference d V) D I K)"
+proof -
+  show ?thesis
+    by (rule exI[of _ assembled.framed], rule exI[of _ assembled.literals], rule exI[of _ assembled.callees],
+        rule exI[of _ assembled.interior], rule exI[of _ assembled.slots])
+       (use assembled.frame.record_formed assembled.frame.record_counts assembled.frame.record_root
+          assembled.reference_table assembled.carrier assembled.boundary assembled.reference_domain deps recover in blast)
+qed
+
+end
+
 theorem inference_node_syntax_total:
   fixes d :: "local_address option definition_site"
     and V :: "(local_address option definition_site \<times> factor_term) fset"
@@ -36,120 +178,22 @@ proof -
     "\<forall>E u. environment_formed E \<longrightarrow> artifact_at E u Rp \<longrightarrow> syntax_references E u Lp Cp \<longrightarrow>
       native_discharge_table_at E u [] D Ip Kp"
     using discharge_table_syntax_total[OF dfinite dfunctional endpoints] by blast
-  let ?Rc = "external_occurrence_syntax (snd d)"
-  let ?Ci = "{[],[5]} :: local_address set"
-  let ?Ck = "{[4]} :: local_address set"
-  let ?Cs = "[{([4],d)},Cb,Cp]"
-  let ?Ls = "[{},Lb,Lp]"
-  let ?Is = "[?Ci,Ib,Ip]"
-  let ?Ks = "[?Ck,Kb,Kp]"
-  let ?Rs = "[?Rc,Rb,Rp]"
-  have cf: "exact_formed ?Rc" by (rule external_occurrence_syntax_formed[OF address])
-  have profile: "reference_table_formed {} {([4],d)}"
-    by (rule reference_table_callees) (simp_all add: single_valued_def)
-  have cc: "rra_carrier (object_structure ?Rc)=?Ci\<union>?Ck"
-    by (auto simp: external_occurrence_syntax_def)
-  have cs: "?Ci\<inter>?Ck={}" by auto
-  have cd: "?Ck=rel_dom ({} :: (local_address\<times>exact_artifact) set)\<union>rel_dom {([4],d)}"
-    by (auto simp: rel_dom_def)
-  interpret assembled: record_syntax_construction ?Rs ?Is ?Ks ?Ls ?Cs
-  proof (rule record_syntax_construction.intro)
-    show "\<forall>R\<in>set ?Rs. exact_formed R" using cf b(1) p(1) by simp
-    show "\<forall>R\<in>set ?Rs. bag_count (object_data R)=(\<lambda>_. 0)"
-      using b(2) p(2) external_occurrence_syntax_properties(2) by simp
-    show "\<forall>R\<in>set ?Rs. []\<in>rra_carrier (object_structure R)"
-      using b(3) p(3) external_occurrence_syntax_properties(1) by simp
-    show "length ?Is=length ?Rs" "length ?Ks=length ?Rs"
-      "length ?Ls=length ?Rs" "length ?Cs=length ?Rs" by simp_all
-    show "\<forall>i<length ?Rs. rra_carrier (object_structure (?Rs!i))=?Is!i\<union>?Ks!i"
-      using cc b(5) p(5) by (auto simp: less_Suc_eq)
-    show "\<forall>i<length ?Rs. ?Is!i\<inter>?Ks!i={}"
-      using cs b(6) p(6) by (auto simp: less_Suc_eq)
-    show "\<forall>i<length ?Rs. ?Ks!i=rel_dom (?Ls!i)\<union>rel_dom (?Cs!i)"
-      using cd b(7) p(7) by (auto simp: less_Suc_eq)
-    show "\<forall>i<length ?Rs. reference_table_formed (?Ls!i) (?Cs!i)"
-      using profile b(4) p(4) by (auto simp: less_Suc_eq)
-  qed
-  have br: "rel_dom Lb\<union>rel_dom Cb\<subseteq>rra_carrier (object_structure Rb)" using b(5,7) by blast
-  have pr: "rel_dom Lp\<union>rel_dom Cp\<subseteq>rra_carrier (object_structure Rp)" using p(5,7) by blast
-  have bd: "rel_dom (fset V)\<subseteq>rel_ran Cb" using b(8) by simp
-  have pd: "rel_dom D\<union>rel_ran D\<subseteq>rel_ran Cp" using p(8) by simp
-  have cite_range: "rel_ran {([4],d)}={d}" by (auto simp: rel_ran_def)
-  have deps: "rel_ran assembled.callees=insert d (rel_dom (fset V)\<union>rel_dom D\<union>rel_ran D)"
-    using assembled.reference_range by (simp add: cite_range b(8) p(8) Un_assoc)
-  have recover: "\<forall>E u. environment_formed E \<longrightarrow> artifact_at E u assembled.framed \<longrightarrow>
-      syntax_references E u assembled.literals assembled.callees \<longrightarrow>
-      native_proof_node_at E u [] (Schema_Inference d V) D assembled.interior assembled.slots"
-  proof (intro allI impI)
-    fix E u assume ef: "environment_formed E" and art: "artifact_at E u assembled.framed"
-      and refs: "syntax_references E u assembled.literals assembled.callees"
-    have caddr: "finite_addressing (rra_carrier (object_structure ?Rc)) (syntax_branch 0)"
-      using assembled.child_addressing[of 0] by simp
-    have cread: "object_reads_agree (push_object (syntax_branch 0) ?Rc) assembled.framed
-      (image (syntax_branch 0) (rra_carrier (object_structure ?Rc)))"
-      using assembled.frame.record_child_reads[of 0] by simp
-    have centry: "(syntax_branch 0 [4],d)\<in>assembled.callees"
-      by (rule syntax_forest_table_member[where i=0]) simp_all
-    have cite: "site_citation_at E u (syntax_branch 0 []) d (image (syntax_branch 0) ?Ci) {syntax_branch 0 [4]}"
-      by (rule external_syntax_embedded_site[OF ef art address caddr cread refs centry])
-    have baddr: "finite_addressing (rra_carrier (object_structure Rb)) (syntax_branch 1)"
-      using assembled.child_addressing[of 1] by simp
-    have bread: "object_reads_agree (push_object (syntax_branch 1) Rb) assembled.framed
-      (image (syntax_branch 1) (rra_carrier (object_structure Rb)))"
-      using assembled.frame.record_child_reads[of 1] by simp
-    have brefs: "syntax_references E u (map_slot_keys (syntax_branch 1) Lb) (map_slot_keys (syntax_branch 1) Cb)"
-      using assembled.child_references[OF refs, of 1] by simp
-    have binding_read: "native_binding_table_at E u (syntax_branch 1 []) (fset V)
-      (image (syntax_branch 1) Ib) (image (syntax_branch 1) Kb)"
-      by (rule compiled_binding_table_embedded[OF b(1) br b(9)[rule_format] bd ef art
-          syntax_branch_injective baddr bread brefs])
-    have paddr: "finite_addressing (rra_carrier (object_structure Rp)) (syntax_branch 2)"
-      using assembled.child_addressing[of 2] by simp
-    have pread: "object_reads_agree (push_object (syntax_branch 2) Rp) assembled.framed
-      (image (syntax_branch 2) (rra_carrier (object_structure Rp)))"
-      using assembled.frame.record_child_reads[of 2] by simp
-    have prefs: "syntax_references E u (map_slot_keys (syntax_branch 2) Lp) (map_slot_keys (syntax_branch 2) Cp)"
-      using assembled.child_references[OF refs, of 2] by simp
-    have discharge_read: "native_discharge_table_at E u (syntax_branch 2 []) D
-      (image (syntax_branch 2) Ip) (image (syntax_branch 2) Kp)"
-      by (rule compiled_discharge_table_embedded[OF p(1) pr p(9)[rule_format] pd ef art
-          syntax_branch_injective paddr pread prefs])
-    let ?C = "image (syntax_branch 0) ?Ci"
-    let ?B = "image (syntax_branch 1) Ib"
-    let ?P = "image (syntax_branch 2) Ip"
-    let ?A = "{syntax_branch 0 [4]}"
-    let ?L = "image (syntax_branch 1) Kb"
-    let ?W = "image (syntax_branch 2) Kp"
-    have rec: "record_at assembled.framed [] assembled.frame.ports
-      [syntax_branch 0 [],syntax_branch 1 [],syntax_branch 2 []]"
-      using assembled.frame.record_read by (simp add: upt_conv_Cons numeral_2_eq_2)
-    have header: "insert [] (set assembled.frame.ports)\<inter>(?C\<union>?B\<union>?P)={}"
-      using assembled.header_separate by (simp add: syntax_forest_three_positions Un_assoc)
-    have cb: "?C\<inter>?B={}" using assembled.child_interiors_separate[of 0 1] by simp
-    have cp: "?C\<inter>?P={}" using assembled.child_interiors_separate[of 0 2] by simp
-    have bp: "?B\<inter>?P={}" using assembled.child_interiors_separate[of 1 2] by simp
-    have separate: "insert [] (set assembled.frame.ports\<union>?C\<union>?B\<union>?P)\<inter>(?A\<union>?L\<union>?W)={}"
-      using assembled.boundary by (simp add: syntax_forest_three_positions Un_assoc)
-    have native: "native_proof_node_at E u [] (Schema_Inference d V) D
-      (insert [] (set assembled.frame.ports\<union>?C\<union>?B\<union>?P)) (?A\<union>?L\<union>?W)"
-      by (rule native_proof_node_at.inference[OF ef art rec cite binding_read discharge_read header cb cp bp separate])
-    show "native_proof_node_at E u [] (Schema_Inference d V) D assembled.interior assembled.slots"
-      using native by (simp add: syntax_forest_three_positions Un_assoc)
-  qed
-  show ?thesis
-    by (rule exI[of _ assembled.framed], rule exI[of _ assembled.literals], rule exI[of _ assembled.callees],
-        rule exI[of _ assembled.interior], rule exI[of _ assembled.slots])
-       (use assembled.frame.record_formed assembled.frame.record_counts assembled.frame.record_root
-          assembled.reference_table assembled.carrier assembled.boundary assembled.reference_domain deps recover in blast)
+  interpret construction: inference_node_syntax_construction d V D Rb Rp Lb Lp Cb Cp Ib Kb Ip Kp
+    by (rule inference_node_syntax_construction.intro[OF address b p])
+  show ?thesis by (rule construction.total)
 qed
 
 section \<open>An assertion has an explicit complete empty record\<close>
 
-theorem assertion_node_syntax_total:
-  "\<exists>R. exact_formed R \<and> bag_count (object_data R)=(\<lambda>_. 0) \<and>
-    rra_carrier (object_structure R)={[]} \<and>
-    (\<forall>E u. environment_formed E \<longrightarrow> artifact_at E u R \<longrightarrow>
-      native_proof_node_at E u [] Schema_Assertion {} {[]} {})"
+definition assertion_node_syntax :: exact_artifact where
+  "assertion_node_syntax=record_wrapper (syntax_forest []) [] [] []"
+
+theorem assertion_node_syntax_properties:
+  "exact_formed assertion_node_syntax"
+  "bag_count (object_data assertion_node_syntax)=(\<lambda>_. 0)"
+  "rra_carrier (object_structure assertion_node_syntax)={[]}"
+  "\<forall>E u. environment_formed E \<longrightarrow> artifact_at E u assertion_node_syntax \<longrightarrow>
+    native_proof_node_at E u [] Schema_Assertion {} {[]} {}"
 proof -
   interpret frame: syntax_family_construction "[]" by (rule syntax_family_construction.intro) simp_all
   have carrier: "rra_carrier (object_structure frame.record_framed)={[]}"
@@ -159,9 +203,22 @@ proof -
   have every: "\<forall>E u. environment_formed E \<longrightarrow> artifact_at E u frame.record_framed \<longrightarrow>
       native_proof_node_at E u [] Schema_Assertion {} {[]} {}"
     by (intro allI impI) (rule native_proof_node_at.assertion[OF _ _ rec]; assumption)
-  show ?thesis by (rule exI[of _ frame.record_framed])
-    (use frame.record_formed frame.record_counts carrier every in blast)
+  have same: "assertion_node_syntax=frame.record_framed"
+    by (simp add: assertion_node_syntax_def family_ports_def)
+  show "exact_formed assertion_node_syntax"
+    "bag_count (object_data assertion_node_syntax)=(\<lambda>_. 0)"
+    "rra_carrier (object_structure assertion_node_syntax)={[]}"
+    "\<forall>E u. environment_formed E \<longrightarrow> artifact_at E u assertion_node_syntax \<longrightarrow>
+      native_proof_node_at E u [] Schema_Assertion {} {[]} {}"
+    using frame.record_formed frame.record_counts carrier every by (simp_all only: same)
 qed
+
+theorem assertion_node_syntax_total:
+  "\<exists>R. exact_formed R \<and> bag_count (object_data R)=(\<lambda>_. 0) \<and>
+    rra_carrier (object_structure R)={[]} \<and>
+    (\<forall>E u. environment_formed E \<longrightarrow> artifact_at E u R \<longrightarrow>
+      native_proof_node_at E u [] Schema_Assertion {} {[]} {})"
+  using assertion_node_syntax_properties by blast
 
 text \<open>
   Each inference has an actual three-field record with a clause citation,
