theories/Native_Node_Investigation_Execution.thy
@@ -1,0 +1,13 @@
+theory Native_Node_Investigation_Execution
+  imports Factor_Native_Node_Investigation
+begin
+
+setup \<open>Finite_Observation_Contracts.export @{term native_node_investigation}\<close>
+
+export_code native_node_indices native_node_report_packet native_node_inspect
+  finite_environment_artifact_rows finite_environment_bindings finite_artifact_rows
+  Finite_Inference Finite_Assertion Finite_Target Finite_Payload Finite_Pair Finite_Whole Finite_Anchor
+  fset set nat_of_integer integer_of_nat
+  in SML module_name Native_Node_Investigation_Execution file_prefix native_node_investigation
+
+end
